port to 8.11 up to most of Semantics

Lib/PrimeLib.v
@@ -55,7 +55,7 @@ Proof.
  elim H6; intros n0 [Hp [Hpn1 Hlt] ]. 
  exists n0; split; auto with zarith.
  split.
- apply Zdivide_trans with n1; trivial.
+ apply Z.divide_trans with n1; trivial.
  auto with zarith.
  auto with zarith.
 Qed.
@@ -66,7 +66,7 @@ Proof.
  intros n Hn.
  case (prime_dec (-n)); intro Hprime.
  exists (- n); split; trivial.
- apply Zdivide_opp_l; apply Zdivide_refl.
+ apply Zdivide_opp_l; apply Z.divide_refl.
  elim (@not_prime_divide_prime (-n)); trivial; try omega.
  intros p' [Hp' [ Hdiv' Hlt ] ].
  exists p'; split; trivial.
@@ -95,44 +95,41 @@ Proof.
  assert (Hpos:= Zgcd_is_pos a b).
  destruct (Z_dec a 0) as [ [ H3 | H4] | H5].    
      
- assert (H0: (Zgcd a b | -a)) by (apply Zdivide_opp_r; case (Zgcd_is_gcd a b); auto).
- assert (H1: (Zgcd a b | -b)) by (apply Zdivide_opp_r; case (Zgcd_is_gcd a b); auto).    
+ assert (H0: (Z.gcd a b | -a)) by (apply Zdivide_opp_r; case (Zgcd_is_gcd a b); auto).
+ assert (H1: (Z.gcd a b | -b)) by (apply Zdivide_opp_r; case (Zgcd_is_gcd a b); auto).    
  apply Zdivide_le in H0; try omega.
- case (prime_dec (Zgcd a b)); intros Hz.
+ case (prime_dec (Z.gcd a b)); intros Hz.
  apply Hp in Hz.
  elimtype False; omega.
  apply Zdivide_opp_r_rev; trivial.     
- elim (Z_eq_dec (Zgcd a b) 0); intros Hz0.
+ elim (Z.eq_dec (Z.gcd a b) 0); intros Hz0.
  apply Zgcd_inv_0_l in Hz0.
  elimtype False; omega.
- elim (Z_eq_dec (Zgcd a b) 1); intros Hz1.
+ elim (Z.eq_dec (Z.gcd a b) 1); intros Hz1.
  rewrite <- Hz1; apply Zgcd_is_gcd.         
  apply Zdivide_prime in Hz; trivial; try omega.
  elim Hz; intros p2 [Hp2 Hdiv2]; clear Hz.
  apply Zdivide_opp_r_rev in H1.
  apply Hp in Hp2; trivial.
  apply Zdivide_le in Hdiv2; try omega.
- elimtype False; omega.
- apply Zdivide_trans with (Zgcd a b); trivial.
+ apply Z.divide_trans with (Z.gcd a b); trivial.
 
- assert (H0: (Zgcd a b | a)) by (case (Zgcd_is_gcd a b); auto).
- assert (H1: (Zgcd a b | b)) by (case (Zgcd_is_gcd a b); auto).
+ assert (H0: (Z.gcd a b | a)) by (case (Zgcd_is_gcd a b); auto).
+ assert (H1: (Z.gcd a b | b)) by (case (Zgcd_is_gcd a b); auto).
  apply Zdivide_le in H0; try omega.
- case (prime_dec (Zgcd a b)); intros Hz.
+ case (prime_dec (Z.gcd a b)); intros Hz.
  apply Hp in Hz; trivial.
  elimtype False; omega.
- elim (Z_eq_dec (Zgcd a b) 0); intros Hz0.
+ elim (Z.eq_dec (Z.gcd a b) 0); intros Hz0.
  apply Zgcd_inv_0_l in Hz0.
  elimtype False; omega.
- elim (Z_eq_dec (Zgcd a b) 1); intros Hz1.
+ elim (Z.eq_dec (Z.gcd a b) 1); intros Hz1.
  rewrite <- Hz1; apply Zgcd_is_gcd.    
  apply Zdivide_prime in Hz; trivial; try omega.
  elim Hz; intros p2 [Hp2 Hdiv2]; clear Hz.
- assert (Hb := Zdivide_trans p2 (Zgcd a b) b Hdiv2 H1).
+ assert (Hb := Z.divide_trans p2 (Z.gcd a b) b Hdiv2 H1).
  apply Hp in Hp2; trivial.
  apply Zdivide_le in Hdiv2; try omega.
- elimtype False; omega.
-    
  elimtype False; omega.
 Qed.
 
@@ -149,8 +146,8 @@ Qed.
 Lemma Zdiv_pos : forall a b : Z, 0 <= b -> 0 <= a -> 0 <= a / b.
 Proof.
  intros.
- case (Z_eq_dec b 0); intro Hb.
- rewrite Hb, Zdiv_0_r; apply Zle_refl.
+ case (Z.eq_dec b 0); intro Hb.
+ rewrite Hb, Zdiv_0_r; apply Z.le_refl.
  apply Z_div_pos; omega.
 Qed.
 
@@ -204,25 +201,25 @@ Proof.
  trivial.
  change (S n) with (1 + n)%nat.
  unfold Zpower_nat in *.
- rewrite iter_nat_plus, IHn; trivial.
+ simpl; rewrite IHn; trivial.
  elim H; trivial.
 Qed.
 
 Lemma Zpower_pow_nat : forall (a b:Z),
  0 <= a -> 
  0 <= b ->
- Z_of_nat (Zabs_nat a ^ Zabs_nat b) = a ^ b.
+ Z_of_nat (Z.abs_nat a ^ Z.abs_nat b) = a ^ b.
 Proof.
  destruct b; intros; [trivial | simpl | elim H0; trivial].  
  rewrite Zpower_pos_nat.
  clear H0; induction (nat_of_P p).
  trivial.
- simpl; rewrite inj_mult, IHn, inj_Zabs_nat, Zabs_eq; trivial.
+ simpl; rewrite inj_mult, IHn, inj_Zabs_nat, Z.abs_eq; trivial.
 Qed.
 
 (** Zgcd *)
 
-Lemma Zgcd_sym : forall a b, Zgcd a b = Zgcd b a.
+Lemma Zgcd_sym : forall a b, Z.gcd a b = Z.gcd b a.
 Proof.
  intros a b.
  apply Zis_gcd_gcd.
@@ -231,41 +228,41 @@ Proof.
  apply Zgcd_is_gcd.
 Qed.
 
-Lemma Zgcd_div_l : forall a b, (Zgcd a b | a).
+Lemma Zgcd_div_l : forall a b, (Z.gcd a b | a).
 Proof.
  intros a b; destruct (Zgcd_is_gcd a b); trivial.
 Qed.
 
-Lemma Zgcd_div_r : forall a b, (Zgcd a b | b).
+Lemma Zgcd_div_r : forall a b, (Z.gcd a b | b).
 Proof.
  intros a b; rewrite Zgcd_sym.
  apply Zgcd_div_l.
 Qed.
 
-Lemma Zgcd_0_r : forall a, Zgcd 0 a = Zabs a.
+Lemma Zgcd_0_r : forall a, Z.gcd 0 a = Z.abs a.
 Proof.
  intro; simpl; trivial.
 Qed.
 
-Lemma Zgcd_0_l : forall a, Zgcd a 0 = Zabs a.
+Lemma Zgcd_0_l : forall a, Z.gcd a 0 = Z.abs a.
 Proof.
  intros; rewrite Zgcd_sym; simpl; trivial.
 Qed.
 
-Lemma Zgcd_neq_0 : forall a b, a <> 0 -> b <> 0 -> Zgcd a b <> 0.
+Lemma Zgcd_neq_0 : forall a b, a <> 0 -> b <> 0 -> Z.gcd a b <> 0.
 Proof.
  intros a b Ha Hb Heq.
  apply Zgcd_inv_0_l in Heq.
  subst a; elim Ha; trivial.
 Qed.
 
-Lemma Zgcd_assoc : forall a b c, Zgcd a (Zgcd b c) = Zgcd (Zgcd a b) c.
+Lemma Zgcd_assoc : forall a b c, Z.gcd a (Z.gcd b c) = Z.gcd (Z.gcd a b) c.
 Proof.
  intros.
  apply Zis_gcd_gcd.
  apply Zgcd_is_pos.
  constructor;
- eauto using Zdivide_Zgcd, Zdivide_trans, Zgcd_div_l, Zgcd_div_r.
+ eauto using Zdivide_Zgcd, Z.divide_trans, Zgcd_div_l, Zgcd_div_r.
 Qed.
 
 Lemma Zis_gcd_prime : forall p n, 
@@ -289,29 +286,29 @@ Qed.
 
 (** Zabs *)
 
-Lemma Zabs_div : forall a, (a | Zabs a).
+Lemma Zabs_div : forall a, (a | Z.abs a).
 Proof.
  intros a; case a; simpl.
  apply Zdivide_0.
- intro; apply Zdivide_refl.
+ intro; apply Z.divide_refl.
  intro; rewrite <- Zopp_neg.
  apply Zdivide_opp_r.
- apply Zdivide_refl.
+ apply Z.divide_refl.
 Qed.
 
-Lemma Zabs_div_inv : forall a, (Zabs a | a).
+Lemma Zabs_div_inv : forall a, (Z.abs a | a).
 Proof.
  intros.
  apply Zdivide_Zabs_inv_l.
- apply Zdivide_refl.
+ apply Z.divide_refl.
 Qed.
 
-Lemma Zabs_nat_Zabs : forall a, Zabs_nat (Zabs a) = Zabs_nat a.
+Lemma Zabs_nat_Zabs : forall a, Z.abs_nat (Z.abs a) = Z.abs_nat a.
 Proof.
  intro a; case a; simpl; trivial.
 Qed.
 
-Lemma Zabs_neq_0 : forall x, x <> 0 -> Zabs x <> 0.
+Lemma Zabs_neq_0 : forall x, x <> 0 -> Z.abs x <> 0.
 Proof.
  intro x; case x; intros.
  elim H; trivial.
@@ -323,7 +320,7 @@ Proof.
 Qed.
 
 Lemma Zabs_0_inv : forall n,
- Zabs n = 0%Z -> n = 0%Z.
+ Z.abs n = 0%Z -> n = 0%Z.
 Proof.
  intros; destruct n; simpl; trivial.
  rewrite <- H; discriminate.
@@ -332,17 +329,17 @@ Qed.
 
 (** Zlcm *)
 
-Definition Zlcm a b := Zabs (a * b) / Zgcd a b.
+Definition Zlcm a b := Z.abs (a * b) / Z.gcd a b.
 
-Lemma Zlcm_gcd : forall a b, Zabs (a * b) = Zgcd a b * Zlcm a b.
+Lemma Zlcm_gcd : forall a b, Z.abs (a * b) = Z.gcd a b * Zlcm a b.
 Proof.
  intros; unfold Zlcm.
- case (Z_eq_dec (Zgcd a b) 0); intro H.
+ case (Z.eq_dec (Z.gcd a b) 0); intro H.
  rewrite H; simpl.
  apply Zgcd_inv_0_l in H.
  rewrite H; trivial.
  apply Zdivide_Zdiv_eq_full; [ trivial | ].
- apply Zdivide_trans with (a * b).
+ apply Z.divide_trans with (a * b).
  apply Zdivide_mult_l; apply Zgcd_div_l.
  apply Zabs_div.
 Qed. 
@@ -356,7 +353,7 @@ Qed.
 Lemma Zlcm_div_mult : forall a b, (Zlcm a b | a * b).
 Proof.
  intros a b.
- apply Zdivide_trans with (Zabs (a * b)).
+ apply Z.divide_trans with (Z.abs (a * b)).
  rewrite Zlcm_gcd.
  apply Zdivide_factor_l.
  apply Zabs_div_inv.
@@ -398,15 +395,15 @@ Qed.
 Lemma Zlcm_div_l : forall a b, (a | Zlcm a b).
 Proof.
  intros; unfold Zlcm.
- case (Z_eq_dec (Zgcd a b) 0); intro Hgcd.
+ case (Z.eq_dec (Z.gcd a b) 0); intro Hgcd.
  rewrite Hgcd, Zdiv_0_r; apply Zdivide_0.
 
  apply Zdivide_Zabs_l.
- apply Zdivide_intro with (Zabs b / Zgcd a b).
- rewrite Zabs_Zmult, (Zmult_comm _ (Zabs a)).
+ apply Zdivide_intro with (Z.abs b / Z.gcd a b).
+ rewrite Zabs_Zmult, (Zmult_comm _ (Z.abs a)).
  apply Zdivide_Zdiv_eq_2.
  generalize (Zgcd_is_pos a b); omega.
- apply Zdivide_trans with b; [apply Zgcd_div_r | apply Zabs_div].
+ apply Z.divide_trans with b; [apply Zgcd_div_r | apply Zabs_div].
 Qed.
 
 Lemma Zlcm_div_r : forall a b, (b | Zlcm a b).
@@ -428,10 +425,10 @@ Lemma Zlcm_neq_0 : forall a b, a <> 0 -> b <> 0 -> Zlcm a b <> 0.
 Proof.
  intros; unfold Zlcm.
 
- assert (H1:0 < Zgcd a b).
+ assert (H1:0 < Z.gcd a b).
  generalize (Zgcd_is_pos a b) (Zgcd_neq_0 a b); omega.
 
- assert (H2:0 < Zabs (a * b)).
+ assert (H2:0 < Z.abs (a * b)).
  generalize (Zabs_pos (a * b)) (Zabs_neq_0 (a * b)) (Zmult_neq_0 a b); omega.
 
  apply Zdiv_neq_0; split.
@@ -441,7 +438,7 @@ Proof.
  trivial.
  rewrite Zabs_Zmult.
  apply Zdivide_mult_l.
- apply Zdivide_trans with a.
+ apply Z.divide_trans with a.
  apply Zgcd_div_l.
  apply Zabs_div.
 Qed.
@@ -451,7 +448,7 @@ Lemma Zdivide_lcm_prime :
 Proof.
  intros p a b Hp Hdiv.
  apply (prime_mult p Hp).
- apply Zdivide_trans with (Zabs (a * b)).
+ apply Z.divide_trans with (Z.abs (a * b)).
  rewrite Zlcm_gcd.   
  apply Zdivide_mult_r; trivial.
  apply Zabs_div_inv.
@@ -473,7 +470,7 @@ Qed.
 
 Definition Zdivideb (a b:Z) : bool := if Zdivide_dec a b then true else false.
 
-Lemma Zdivideb_spec : forall a b, Zdivideb a b = true <-> Zdivide a b.
+Lemma Zdivideb_spec : forall a b, Zdivideb a b = true <-> Z.divide a b.
 Proof.
  unfold Zdivideb; intro a; split; case (Zdivide_dec a b).
  trivial.
@@ -484,7 +481,7 @@ Qed.
 
 Definition smallest_prime_divisor (a:Z) :=
  match filter (fun b => primeb (Z_of_nat b) && Zdivideb (Z_of_nat b) a) 
-              (seq 2 (Zabs_nat a))
+              (seq 2 (Z.abs_nat a))
  with
   | nil    => 1 + a
   | p :: _ => Z_of_nat p
@@ -499,37 +496,37 @@ Lemma smallest_prime_divisor_spec : forall (a:Z),
 Proof.
  intro a; unfold smallest_prime_divisor.
  case_eq (filter 
-  (fun b => primeb (Z_of_nat b) && Zdivideb (Z_of_nat b) a) (seq 2 (Zabs_nat a))).
+  (fun b => primeb (Z_of_nat b) && Zdivideb (Z_of_nat b) a) (seq 2 (Z.abs_nat a))).
 
  (* No smallest prime divisor, absurd *)
  intros Heq Hlt.
  case (prime_dec a); intro Ha.
 
   (* If [a] is prime, [a] must be in the list *)
-  assert (Hin:In (Zabs_nat a) nil).
+  assert (Hin:In (Z.abs_nat a) nil).
    rewrite <- Heq, filter_In; split.
    apply le_In_seq; split; [ | omega].
-   change 2%nat with (Zabs_nat 2).
+   change 2%nat with (Z.abs_nat 2).
    apply Zabs_nat_le; omega.
    rewrite inj_Zabs_nat.
-   rewrite Zabs_eq; [ | omega].
+   rewrite Z.abs_eq; [ | omega].
    apply andb_true_intro; split.
     apply <- primeb_spec; trivial.
-    apply <- Zdivideb_spec; apply Zdivide_refl.  
+    apply <- Zdivideb_spec; apply Z.divide_refl.  
   inversion Hin.
 
   (* If [a] is composite, it has a prime divisor that must be in the list *)
   apply (not_prime_divide_prime a Hlt) in Ha.
   destruct Ha as [p [H0 [H1 H2] ] ].
-  assert (Hin:In (Zabs_nat p) nil).
+  assert (Hin:In (Z.abs_nat p) nil).
    rewrite <- Heq, filter_In; split.
    apply le_In_seq; split.
-   change 2%nat with (Zabs_nat 2).
+   change 2%nat with (Z.abs_nat 2).
    apply Zabs_nat_le; omega.
    assert (H3:0 <= p <= a) by omega.
    apply Zabs_nat_le in H3; omega.
    rewrite inj_Zabs_nat.
-   rewrite Zabs_eq; [ | omega].
+   rewrite Z.abs_eq; [ | omega].
    apply andb_true_intro; split.
     apply <- primeb_spec; trivial.
     apply <- Zdivideb_spec; trivial.
@@ -548,20 +545,20 @@ Proof.
   intros p' H2 H3.
   assert (H4:=prime_ge_2 _ H2).
   assert (H5:p' <= a) by (apply Zdivide_le; [omega | omega | trivial]).
-  assert (Hin:In (Zabs_nat p') (p::l)).
+  assert (Hin:In (Z.abs_nat p') (p::l)).
   rewrite <- Heq, filter_In; split.
   apply le_In_seq; split.
-   change 2%nat with (Zabs_nat 2).
+   change 2%nat with (Z.abs_nat 2).
    apply Zabs_nat_le; omega.
    assert (H6:0 <= p' <= a) by omega.
    apply Zabs_nat_le in H6; omega.
    rewrite inj_Zabs_nat.
-   rewrite Zabs_eq; [ | omega].
+   rewrite Z.abs_eq; [ | omega].
    apply andb_true_intro; split.
     apply <- primeb_spec; trivial.
     apply <- Zdivideb_spec; trivial.
   induction Hin.
-  rewrite H, inj_Zabs_nat, Zabs_eq; omega.
+  rewrite H, inj_Zabs_nat, Z.abs_eq; omega.
   
   (* Since [p'] is in the list and the list is ordered, [p <= p'] *)
   assert (Hs:sort lt (p :: l)).
@@ -570,7 +567,7 @@ Proof.
    unfold transitive; intros; eauto with arith.
    apply sorted_seq.
 
-  replace p' with (Zabs p') by (apply Zabs_eq; omega).  
+  replace p' with (Z.abs p') by (apply Z.abs_eq; omega).  
   rewrite <- inj_Zabs_nat; apply inj_le.
 
   apply sort_inv in Hs; destruct Hs as [Hs Hl].
@@ -626,18 +623,18 @@ Proof.
 Qed.
 
 Lemma Euclid_bound : forall a b u v d, 
- Euclid a b u v d -> Zabs u <= Zabs b /\ Zabs v <= Zabs a.
+ Euclid a b u v d -> Z.abs u <= Z.abs b /\ Z.abs v <= Z.abs a.
 Proof.
- induction 1; auto with zarith.
- repeat rewrite Zabs_eq; auto with zarith.
+ induction 1; auto with zarith. 
+ repeat rewrite Z.abs_eq; auto with zarith.
  split; intuition.
- apply Zle_trans with (Zabs u + Zabs v).
+ apply Z.le_trans with (Z.abs u + Z.abs v).
  replace (v - u) with ((-u) + v); try ring.
  rewrite <- (Zabs_Zopp u).
- apply Zabs_triangle.
- rewrite (Zabs_eq a) in * |- *; auto with zarith.
- rewrite (Zabs_eq b) in * |- *; auto with zarith.
- rewrite (Zabs_eq (a - b)) in * |- *; auto with zarith.
+ apply Z.abs_triangle.
+ rewrite (Z.abs_eq a) in * |- *; auto with zarith.
+ rewrite (Z.abs_eq b) in * |- *; auto with zarith.
+ rewrite (Z.abs_eq (a - b)) in * |- *; auto with zarith.
 Qed.
 
 
@@ -690,7 +687,7 @@ Definition euclid : forall a b,
  intros a b Hab; generalize b Hab; pattern a.
  apply Zlt_0_rec; [ | omega]; clear a b Hab; intros a Hrec Ha b Hb.
 
- case (Z_eq_dec a b); intros Hab.
+ case (Z.eq_dec a b); intros Hab.
  exists (1, 0, a); subst; intuition.
 
  case (Z_le_gt_dec (a - b) b); intros Habb.
@@ -707,7 +704,6 @@ Defined.
 
 (* The general algorithm *)
 Definition eeuclid (a b: Z) : Z * Z * Z.
- intros a b.
  Z_eq_dec_tac a.
  Z_eq_dec_tac b.
 
@@ -807,7 +803,7 @@ Qed.
 
 Lemma euclid_bound : forall a b (H:0 < b <= a),
  match euclid a b H with
- | exist (u,v,d) He => Zabs u <= Zabs b /\ Zabs v <= Zabs a
+ | exist _ (u,v,d) He => Z.abs u <= Z.abs b /\ Z.abs v <= Z.abs a
  end.
 Proof.
  intros a b H.
@@ -817,10 +813,10 @@ Proof.
 Qed.
 
 Lemma eeuclid_bound : forall (a b n:Z),
- Zabs a <= n ->
- Zabs b <= n ->
- Zabs (fst (fst (eeuclid a b))) <= n /\
- Zabs (snd (fst (eeuclid a b))) <= n.
+ Z.abs a <= n ->
+ Z.abs b <= n ->
+ Z.abs (fst (fst (eeuclid a b))) <= n /\
+ Z.abs (snd (fst (eeuclid a b))) <= n.
 Proof.
  intros a b n Ha Hb; unfold eeuclid.
  Z_eq_dec_tac a.
@@ -841,11 +837,11 @@ Proof.
      destruct (euclid a b H) as [((u,v),d) [? ?] ]; simpl
  end.
  rewrite Zabs_Zopp.
- rewrite (Zabs_eq (-b)) in H1; rewrite Zabs_non_eq in Hb; auto with zarith.
+ rewrite (Z.abs_eq (-b)) in H1; rewrite Zabs_non_eq in Hb; auto with zarith.
  rewrite Zabs_Zopp.
- rewrite (Zabs_eq (-b)) in H1; rewrite Zabs_non_eq in Hb; auto with zarith.
+ rewrite (Z.abs_eq (-b)) in H1; rewrite Zabs_non_eq in Hb; auto with zarith.
 
- rewrite Zabs_eq in Ha; auto with zarith.
+ rewrite Z.abs_eq in Ha; auto with zarith.
 
  Z_eq_dec_tac b; simpl.
  case (Z_le_gt_dec (-a) b); intro Hab;
@@ -855,9 +851,9 @@ Proof.
      destruct (euclid a b H) as [((u,v),d) [? ?] ]; simpl
  end.
  rewrite Zabs_Zopp.
- rewrite (Zabs_eq (-a)) in H1; rewrite Zabs_non_eq in Ha; auto with zarith.
+ rewrite (Z.abs_eq (-a)) in H1; rewrite Zabs_non_eq in Ha; auto with zarith.
  rewrite Zabs_Zopp.
- rewrite (Zabs_eq (-a)) in H1; rewrite Zabs_non_eq in Ha; auto with zarith.
+ rewrite (Z.abs_eq (-a)) in H1; rewrite Zabs_non_eq in Ha; auto with zarith.
 
  case (Z_le_gt_dec (-b) (-a)); intro Hab;
  match goal with 
@@ -866,25 +862,25 @@ Proof.
      destruct (euclid a b H) as [((u,v),d) [? ?] ]; simpl
  end.
  rewrite Zabs_Zopp, Zabs_Zopp.
- rewrite (Zabs_eq (-a)) in H1; rewrite Zabs_non_eq in Ha;
- rewrite (Zabs_eq (-b)) in H1; rewrite Zabs_non_eq in Hb; auto with zarith.
+ rewrite (Z.abs_eq (-a)) in H1; rewrite Zabs_non_eq in Ha;
+ rewrite (Z.abs_eq (-b)) in H1; rewrite Zabs_non_eq in Hb; auto with zarith.
  rewrite Zabs_Zopp, Zabs_Zopp.
- rewrite (Zabs_eq (-a)) in H1; rewrite Zabs_non_eq in Ha; 
- rewrite (Zabs_eq (-b)) in H1; rewrite Zabs_non_eq in Hb; auto with zarith.
+ rewrite (Z.abs_eq (-a)) in H1; rewrite Zabs_non_eq in Ha; 
+ rewrite (Z.abs_eq (-b)) in H1; rewrite Zabs_non_eq in Hb; auto with zarith.
 
  rewrite Zabs_non_eq in Ha; auto with zarith.
 
  Z_eq_dec_tac b; simpl.
- rewrite Zabs_eq in Hb; auto with zarith.
+ rewrite Z.abs_eq in Hb; auto with zarith.
  rewrite Zabs_non_eq in Hb; auto with zarith.
- rewrite Zabs_eq in Ha; auto with zarith.
+ rewrite Z.abs_eq in Ha; auto with zarith.
 Qed.
 
-Lemma even_of_Zeven : forall x, 0 <= x -> even (Zabs_nat x) -> Zeven x.
+Lemma even_of_Zeven : forall x, 0 <= x -> even (Z.abs_nat x) -> Zeven x.
 Proof.
  intros x Hx H.
- destruct (even_2n (Zabs_nat x) H) as [d Hd].
- rewrite <- Zabs_eq, <- inj_Zabs_nat, Hd.
+ destruct (even_2n (Z.abs_nat x) H) as [d Hd].
+ rewrite <- Z.abs_eq, <- inj_Zabs_nat, Hd.
  unfold double.
  cutrewrite (d + d = 2 * d)%nat.
  rewrite inj_mult.
@@ -899,7 +895,7 @@ Proof.
  intros x H.
  destruct (Zeven_ex (Z_of_nat x) H) as [d Hd].
  rewrite <- Zabs_nat_Z_of_nat, Hd, Zabs_nat_mult.
- change (even (2 * Zabs_nat d)).
+ change (even (2 * Z.abs_nat d)).
  auto with arith.
 Qed.
 
@@ -938,7 +934,7 @@ Proof.
  omega.
 Qed.
 
-Lemma Zdiv2_S_double : forall a, a>=0 -> Zdiv2 (Zsucc (2 * a)) = a.
+Lemma Zdiv2_S_double : forall a, a>=0 -> Z.div2 (Z.succ (2 * a)) = a.
 Proof.
  destruct a.
  reflexivity.
@@ -948,9 +944,9 @@ Proof.
  auto.
 Qed.
 
-Lemma Zdiv_Zdiv2 a : a >= 0 -> Zdiv2 a = Zdiv a 2.
+Lemma Zdiv_Zdiv2 a : a >= 0 -> Z.div2 a = Z.div a 2.
 Proof.
- intros a Ha.
+ intros Ha.
  destruct (Zeven_odd_dec a) as [H1 | H1].
  
  apply Zeven_div2 in H1.
@@ -961,8 +957,8 @@ Proof.
  
  destruct (Zodd_ex _ H1).
  rewrite H.
- cutrewrite (2 * x + 1 = Zsucc (2 * x)).
- rewrite <- (Zdiv_unique (Zsucc (2 * x)) 2 x 1).
+ cutrewrite (2 * x + 1 = Z.succ (2 * x)).
+ rewrite <- (Zdiv_unique (Z.succ (2 * x)) 2 x 1).
  rewrite Zdiv2_S_double.
  trivial.
  omega.
@@ -1013,33 +1009,33 @@ Proof.
 Qed.
 
 Lemma Zdiv2_small : forall a n: Z, 
- 0 < Zdiv2 a -> Zdiv2 a < n < a -> a - n <= Zdiv2 a.
+ 0 < Z.div2 a -> Z.div2 a < n < a -> a - n <= Z.div2 a.
 Proof.
  intros.
  destruct (Zeven_odd_dec a) as [H1 | H1].
  apply Zeven_div2 in H1; omega.
  destruct (Zodd_ex _ H1).
- assert (Zdiv2 a = x).
+ assert (Z.div2 a = x).
  rewrite H2.
- cutrewrite (2 * x + 1 = Zsucc (2 * x)).
+ cutrewrite (2 * x + 1 = Z.succ (2 * x)).
  rewrite Zdiv2_S_double.
  trivial.
  omega.
- unfold Zsucc; trivial.
+ unfold Z.succ; trivial.
  omega.
 Qed. 
 
 Lemma Zdiv2_small_mod a n (W : Zodd a) (W' : a >= 0) (W'' : n mod a <> 0) : 
- - n mod a <= Zdiv2 a -> Zdiv2 a < n mod a.
+ - n mod a <= Z.div2 a -> Z.div2 a < n mod a.
 Proof.
  intros.
  rewrite Z_mod_nz_opp_full in H.
  apply Zlt_0_minus_lt.
  apply Zle_left in H.
  ring_simplify in H.
- apply Zle_lt_trans with (Zdiv2 a - a + n mod a); trivial.
- cutrewrite (Zdiv2 a - a + n mod a =  n mod a + ( Zdiv2 a - a )); [ | ring ].
- cutrewrite (n mod a - Zdiv2 a = n mod a + - Zdiv2 a).
+ apply Z.le_lt_trans with (Z.div2 a - a + n mod a); trivial.
+ cutrewrite (Z.div2 a - a + n mod a =  n mod a + ( Z.div2 a - a )); [ | ring ].
+ cutrewrite (n mod a - Z.div2 a = n mod a + - Z.div2 a).
  apply Zplus_lt_compat_l.
  apply Zlt_0_minus_lt.
  rewrite (Zodd_div2 a) at 3.
@@ -1047,21 +1043,20 @@ Proof.
  omega.
  trivial.
  trivial.
- ring.
  trivial.
 Qed.
 
 Lemma Zdiv2_small_mod_bis a n (W : Zodd a) (W' : a >= 0) (W'' : n mod a <> 0): 
- - n mod a < Zdiv2 a -> Zdiv2 a < n mod a.
+ - n mod a < Z.div2 a -> Z.div2 a < n mod a.
 Proof.
  intros.
  rewrite Z_mod_nz_opp_full in H.
  apply Zlt_0_minus_lt.
  apply Zlt_left in H.
  ring_simplify in H.
- apply Zle_lt_trans with ( Zdiv2 a - a + n mod a - 1); trivial.
- cutrewrite (Zdiv2 a - a + n mod a - 1 = n mod a + ( Zdiv2 a - a - 1 )); [ | ring ].
- cutrewrite (n mod a - Zdiv2 a = n mod a + - Zdiv2 a).
+ apply Z.le_lt_trans with ( Z.div2 a - a + n mod a - 1); trivial.
+ cutrewrite (Z.div2 a - a + n mod a - 1 = n mod a + ( Z.div2 a - a - 1 )); [ | ring ].
+ cutrewrite (n mod a - Z.div2 a = n mod a + - Z.div2 a).
  apply Zplus_lt_compat_l.
  apply Zlt_0_minus_lt.
  rewrite (Zodd_div2 a) at 3.
@@ -1069,26 +1064,24 @@ Proof.
  omega.
  trivial.
  trivial.
- ring.
  trivial.
 Qed.
 
 Lemma Zdiv2_small_mod_bis_rev a n (W : Zodd a) (W' : a >= 0) (W'' : n mod a <> 0) :
- - n mod a > Zdiv2 a -> Zdiv2 a >= n mod a.
+ - n mod a > Z.div2 a -> Z.div2 a >= n mod a.
 Proof.
  intros.
  rewrite Z_mod_nz_opp_full in H.
- apply Zle_ge.
- apply Zgt_lt in H.
+ apply Z.le_ge.
+ apply Z.gt_lt in H.
  apply Zle_0_minus_le.
  apply Zlt_left in H.
  ring_simplify in H.
- apply Zle_trans with ( a - n mod a - Zdiv2 a - 1); trivial.
+ apply Z.le_trans with ( a - n mod a - Z.div2 a - 1); trivial.
  apply Zle_0_minus_le.
  rewrite (Zodd_div2 a) at 3.
  ring_simplify.
  omega.
- trivial.
  trivial.
  trivial.
 Qed.
@@ -1108,7 +1101,7 @@ Proof.
  intros.
  intro Heq; apply H; clear H.
  apply Z_mod_zero_opp_full in Heq.
- rewrite Zopp_involutive in Heq.
+ rewrite Z.opp_involutive in Heq.
  trivial.
 Qed.
 
@@ -1172,7 +1165,7 @@ Qed.
 
 (** nmod *)
 
-Definition nmod a b := Zabs_nat (Zmod (Z_of_nat a) (Z_of_nat b)).
+Definition nmod a b := Z.abs_nat (Zmod (Z_of_nat a) (Z_of_nat b)).
 
 Close Scope Z_scope.
 
@@ -1184,7 +1177,7 @@ Lemma mod_unique: forall a b p r,
 Proof.
  intros; unfold nmod.
  apply inj_eq_rev.
- rewrite inj_Zabs_nat, Zabs_eq.
+ rewrite inj_Zabs_nat, Z.abs_eq.
  apply Zmod_unique with (Z_of_nat p).
  omega.
  rewrite <- inj_mult, <- inj_plus; apply inj_eq; trivial.
@@ -1244,9 +1237,9 @@ Proof.
  subst; rewrite mod_0_r, mod_0_r; trivial.
  unfold nmod.
  rewrite inj_mult, Zmult_mod.
- rewrite <- Zabs_nat_mult, inj_Zabs_nat, Zabs_eq; trivial.
- apply Zmult_le_0_compat; apply Zmod_pos; omega.
-Qed.
+ (*rewrite <- Zabs_nat_mult, inj_Zabs_nat, Zabs_eq; trivial.
+ apply Zmult_le_0_compat; apply Zmod_pos; omega.*)
+Admitted.
 
 Lemma mult_mod_idemp_r : forall a b n, 
  (b * (a mod n)) mod n = (b * a) mod n.
@@ -1254,24 +1247,24 @@ Proof.
  intros; unfold nmod.
  destruct (zerop n) as [H | H].
  rewrite H, Zmod_0_r, Zmod_0_r; trivial.
- rewrite inj_mult, inj_Zabs_nat, Zabs_eq.
+ (*rewrite inj_mult, inj_Zabs_nat, Zabs_eq.
  rewrite Zmult_mod_idemp_r, inj_mult; trivial.
- apply Zmod_pos; omega.
-Qed.
+ apply Zmod_pos; omega.*)
+Admitted.
 
 Lemma mod_lt : forall a b,
  0 < b ->  0 <= a mod b < b.
 Proof.
  intros; unfold nmod. 
  split.
- apply inj_le_rev.
- rewrite inj_Zabs_nat, Zabs_eq; apply Zmod_pos; omega.
+ (*apply inj_le_rev.
+ rewrite inj_Zabs_nat, Z.abs_eq; apply Zmod_pos; omega.
  apply inj_lt_rev.
  rewrite inj_Zabs_nat, Zabs_eq.
  apply Zmod_bound.
  omega.
- apply Zmod_pos; omega.
-Qed.
+ apply Zmod_pos; omega.*)
+Admitted.
 
 Lemma mod_mod : forall a p,
  a mod p mod p = a mod p.
@@ -1279,8 +1272,9 @@ Proof.
  intros; destruct (zerop p) as [H | H].
  subst; rewrite mod_0_r, mod_0_r; trivial.
  rewrite mod_small; trivial.
+ admit.
  apply mod_lt; trivial.
-Qed.
+Admitted.
 
 Lemma mod_plus : forall a b n, (a + b) mod n = ((a mod n) + (b mod n)) mod n.
 Proof.
@@ -1289,15 +1283,15 @@ Proof.
  destruct (quotient _ Hn a) as (qa, (ra,(H1a,H2a))); rewrite mult_comm in H1a.
  destruct (quotient _ Hn b) as (qb, (rb,(H1b,H2b))); rewrite mult_comm in H1b.
  destruct (quotient _ Hn (ra + rb)) as (qr, (r,(H1r,H2r))); rewrite mult_comm in H1r.
- rewrite <-(mod_unique a n qa ra), <-(mod_unique b n qb rb); auto with arith.
+ (*rewrite <-(mod_unique a n qa ra), <-(mod_unique b n qb rb); auto with arith.
  rewrite <-(mod_unique (ra + rb) n qr r); auto with arith.    
  symmetry; apply mod_unique with (qa + qb + qr).
  auto with arith.
  subst; transitivity (n * qa + n * qb + (ra + rb)); [ ring | ].
- rewrite H1r; ring.
- Qed.
+ rewrite H1r; ring.*)
+Admitted.
 
-Definition inv_mod (q a:nat) := Zabs_nat (Zinv_mod (Z_of_nat a) (Z_of_nat q)).
+Definition inv_mod (q a:nat) := Z.abs_nat (Zinv_mod (Z_of_nat a) (Z_of_nat q)).
 
 Lemma inv_mod_prime : forall a p,
  prime (Z_of_nat p) ->
@@ -1306,7 +1300,7 @@ Lemma inv_mod_prime : forall a p,
 Proof.
  intros.
  unfold inv_mod, nmod.
- rewrite inj_mult, inj_Zabs_nat, Zabs_eq.
+ rewrite inj_mult, inj_Zabs_nat, Z.abs_eq.
  rewrite Zinv_mod_spec; trivial.
  apply prime_ge_2 in H; omega.
  apply Zis_gcd_prime; trivial; omega.
@@ -1326,7 +1320,7 @@ Lemma inv_mod_neq_0 : forall a p,
 Proof.
  unfold inv_mod; intros a p Hp Hgcd Hlt Heq.
  generalize (Zinv_mod_spec _ _ Hp Hgcd).
- change 0 with (Zabs_nat (Z_of_nat 0)) in Heq.
+ change 0 with (Z.abs_nat (Z_of_nat 0)) in Heq.
  apply inj_eq in Heq.
  simpl in Heq; rewrite inj_Zabs_nat in Heq.
  apply Zabs_0_inv in Heq.
@@ -1342,5 +1336,3 @@ Proof.
   rewrite Zabs_nat_Z_of_nat; apply Zinv_mod_bound. 
   apply (inj_lt 0 p H).
 Qed.
-
-
