Semantics/Dlist.v
@@ -57,7 +57,7 @@ Section DLIST.
   Fixpoint DIn (l:list A) (dl:dlist l) {struct dl}: Prop :=
    match dl with 
    | dnil => False
-   | dcons a' l y dl => eq_dep A P a x a' y \/ DIn dl
+   | dcons y dl => eq_dep A P a x _ y \/ DIn dl
    end.
 
  End DIN.
@@ -68,7 +68,7 @@ Section DLIST.
  Fixpoint dforallb (l:list A) (dl:dlist l) : bool := 
   match dl with 
   | dnil => true
-  | dcons a l pa dl => if f pa then dforallb dl else false
+  | dcons pa dl => if f pa then dforallb dl else false
   end.
 
  Lemma dforallb_forall: forall (l : list A) (dl:dlist l),
@@ -95,8 +95,8 @@ Section DMAP.
 
  Fixpoint dmap (l:list A) (dl: dlist P1 l) {struct dl} : dlist P2 l :=  
   match dl as t0 in (dlist _ l0) return (dlist P2 l0) with
-  | dnil => dnil P2
-  | dcons a l pa dl  => dcons a (f pa) (dmap dl)
+  | dnil _ => dnil P2
+  | dcons l pa dl  => dcons _ (f pa) (dmap dl)
   end.
 
 End DMAP.
@@ -111,8 +111,8 @@ Section DFORALL2.
   (la:list A) (dla : dlist PA la) 
   (lb:list B) (dlb : dlist PB lb) {struct dla} : bool :=
   match dla, dlb with
-  | dnil, dnil => true
-  | dcons a la pa dla, dcons b lb pb dlb =>
+  | dnil _, dnil _ => true
+  | dcons a pa dla, dcons lb pb dlb =>
      if f pa pb then dforall2 dla dlb
      else false
   | _, _ => false
@@ -127,8 +127,8 @@ Section DFOLD_RIGHT.
 
  Fixpoint dfold_right (l:list B) (dlb : dlist P l) {struct dlb} : A :=
   match dlb with
-  | dnil => a0
-  | dcons b l pb dlb => f pb (dfold_right dlb)
+  | dnil _ => a0
+  | dcons l pb dlb => f pb (dfold_right dlb)
   end.
 
 End DFOLD_RIGHT.
@@ -141,8 +141,8 @@ Section DFOLD_LEFT.
 
  Fixpoint dfold_left (l:list B) (dlb : dlist P l) (a0:A) {struct dlb} : A :=
   match dlb with
-  | dnil => a0
-  | dcons b l pb dlb => dfold_left dlb (f a0 pb)
+  | dnil _ => a0
+  | dcons l pb dlb => dfold_left dlb (f a0 pb)
   end.
 
 End DFOLD_LEFT.
@@ -160,8 +160,8 @@ Module MakeDep (EB:EQBOOL_LEIBNIZ).
   Qed.
 
  End Dec.
- 
- Module Dep := DecidableEqDepSet Dec.
+
+ Module Dep := DecidableEqDep Dec.
 
  Module LDec.
 
@@ -180,6 +180,6 @@ Module MakeDep (EB:EQBOOL_LEIBNIZ).
 
  End LDec.
 
- Module LDep := DecidableEqDepSet Dec.
+ Module LDep := DecidableEqDep Dec.
 
 End MakeDep.
